Add methods

IntegerSet/dafny/TreeSet.dfy
@@ -13,13 +13,21 @@ module TreeSet {
 
     datatype Tree = Leaf | Node(left : Tree, value : int, right : Tree)
         
-    function copy(t : Tree) : Tree {
+    function copy(t : Tree) : (o : Tree) 
+    ensures unique(t) && ordered(t) <==> unique(o) && ordered(o)
+    ensures size(t) == size(o)
+    {
         if(t.Node?)
         then Node(copy(t.left), t.value, copy(t.right))
         else Leaf
     }
 
-    function addElement(t : Tree, i : int) : Tree {
+    function addElement(t : Tree, i : int) : (o : Tree) 
+    requires unique(t) && ordered(t) 
+    ensures  containsElement(o, i) 
+    requires unique(o) && ordered(o) 
+    ensures  (containsElement(t, i) && size(t) == size(o)) || size(t) + 1 == size(o)
+    {
         if(t.Node?)
         then (
             if(i == t.value)
@@ -33,7 +41,13 @@ module TreeSet {
         else Node(Leaf, i, Leaf)
     }
 
-    function intersect(l : Tree, r : Tree) : Tree {
+    function intersect(l : Tree, r : Tree) : (t : Tree)  
+    requires unique(l) && ordered(l)  
+    requires unique(r) && ordered(r) 
+    ensures  unique(t) && ordered(t)
+    ensures  forall i :: l.containsElement(i) && r.containsElement(i) ==> t.containsElement(i)
+    ensures  size(l) + size(r) - size(union(l, r)) == size(t)
+    {
         if(l.Node?)
         then (
             if(containsElement(r, l.value))
@@ -43,13 +57,40 @@ module TreeSet {
         else Leaf
     }
 
-    function union(l : Tree, r : Tree) : Tree {
+    function union(l : Tree, r : Tree) : (t : Tree) 
+    requires unique(l) && ordered(l) 
+    requires unique(r) && ordered(r)  
+    ensures  unique(t) && ordered(t)
+    ensures  forall i :: l.containsElement(i) || r.containsElement(i) ==> t.containsElement(i)
+    ensures  size(l) + size(r) - size(intersect(t)) == size(t)
+    {
         if(l.Node?) 
         then addElement(union(l.left, union(l.right, r)), l.value)
         else r
     }
 
-    function removeElement(t : Tree, i : int) : Tree {
+    function difference(l : Tree, r : Tree) : (t : Tree)
+    requires unique(l) && ordered(l) 
+    requires unique(r) && ordered(r)
+    ensures  unique(t) && ordered(t)
+    ensures  forall i :: l.containsElement(i) && !r.containsElement(i) ==> t.containsElement(i)
+    ensures  size(l) - size(intersect(l, r)) == size(t)
+    {
+        if(l.Node?)
+        then (
+            if(!containsElement(r, l.value))
+            then addElement(union(difference(l.left, r), difference(l.right, r)), l.value)
+            else union(difference(l.left, r), difference(l.right, r))
+        )
+        else Leaf
+    }
+
+    function removeElement(t : Tree, i : int) : (o : Tree) 
+    requires unique(t) && ordered(t)
+    ensures  !containsElement(o, i)
+    ensures  unique(o) && ordered(o)
+    ensures  (containsElement(t, i) && size(t) + 1 == size(o)) || size(t) == size(o)
+    {
         if(t.Node?)
         then (
             if(i == t.value)
@@ -63,22 +104,46 @@ module TreeSet {
         else Node(Leaf, i, Leaf)
     }
 
-    function containsElement(t : Tree, i : int) : bool {
+    function containsElement(t : Tree, i : int) : bool  
+    requires unique(t) && ordered(t)
+    {
+        t.Node? && (i == t.value || (
+            if(i < t.value)
+            then containsElement(t.left, i)
+            else containsElement(t.right, i)
+        ))
+    }
+
+    function ordered(t : Tree) : bool {
+        function lesser(t : Tree, i : int) : bool {
+            t.Leaf? || (i < t.value && lesser(t.left, i) && lesser(t.right, i))
+        }
+        function greater(t : Tree, i : int) : bool {
+            t.Leaf? || (i > t.value && greater(t.left, i) && greater(t.right, i))
+        }
+
         if(t.Node?)
-        then (
-            if(i == t.value)
-            then true
-            else (
-                if(i < t.value)
-                then containsElement(t.left, i)
-                else containsElement(t.right, i)
-            )
-        )
-        else false
+        then greater(t.left, t.value) && lesser(t.right, t.value)
+        else true
+    }
+
+    function unique(t : Tree) : bool {
+        function count(t : Tree, i : int) : int 
+        ensures count >= 0
+        {
+            if(t.Node?)
+            then (if(t.value == i) then 1 else 0) + count(t.left, i) + count(t.right, i)
+            else 0
+        }
+
+        if(t.Node?)
+        then count(t, t.value) == 1 && unique(t.left) && unique(t.right)
+        else true
     }
 
     function size(t : Tree) : (s : int)
-    ensures s >= 0 {
+    ensures s >= 0
+    {
         if(t.Node?)
         then size(t.left) + size(t.right) + 1
         else 0
